heap_lang/sugar.v
@@ -21,27 +21,25 @@ Delimit Scope lang_scope with L.
 Bind Scope lang_scope with expr.
 Arguments wp {_ _} _ _%L _.
 (* TODO: The levels are all random. Also maybe we should not
-   make 'new' a keyword. What about Arguments for hoare triples?
-   Also find better notation for function application. Or maybe
-   we can make "App" a coercion from expr to (expr → expr)? *)
-(* The colons indicate binders. *)
+   make 'new' a keyword. What about Arguments for hoare triples?. *)
+(* The colons indicate binders. "let" is not consistent here though,
+   thing are only bound in the "in". *)
 Notation "'rec::' e" := (Rec e) (at level 100) : lang_scope.
 Notation "'λ:' e" := (Lam e) (at level 100) : lang_scope.
-Infix "$" := App : lang_scope.
 Notation "'let:' e1 'in' e2" := (Let e1 e2) (at level 70) : lang_scope.
 Notation "e1 ';' e2" := (Seq e1 e2) (at level 70) : lang_scope.
 Notation "'if' e1 'then' e2 'else' e3" := (If e1 e2 e3) : lang_scope.
 
-Notation "'#0'" := (Var 0) (at level 10) : lang_scope.
-Notation "'#1'" := (Var 1) (at level 10) : lang_scope.
-Notation "'#2'" := (Var 2) (at level 10) : lang_scope.
-Notation "'#3'" := (Var 3) (at level 10) : lang_scope.
-Notation "'#4'" := (Var 4) (at level 10) : lang_scope.
-Notation "'#5'" := (Var 5) (at level 10) : lang_scope.
-Notation "'#6'" := (Var 6) (at level 10) : lang_scope.
-Notation "'#7'" := (Var 7) (at level 10) : lang_scope.
-Notation "'#8'" := (Var 8) (at level 10) : lang_scope.
-Notation "'#9'" := (Var 9) (at level 10) : lang_scope.
+Notation "#0" := (Var 0) (at level 0) : lang_scope.
+Notation "#1" := (Var 1) (at level 0) : lang_scope.
+Notation "#2" := (Var 2) (at level 0) : lang_scope.
+Notation "#3" := (Var 3) (at level 0) : lang_scope.
+Notation "#4" := (Var 4) (at level 0) : lang_scope.
+Notation "#5" := (Var 5) (at level 0) : lang_scope.
+Notation "#6" := (Var 6) (at level 0) : lang_scope.
+Notation "#7" := (Var 7) (at level 0) : lang_scope.
+Notation "#8" := (Var 8) (at level 0) : lang_scope.
+Notation "#9" := (Var 9) (at level 0) : lang_scope.
 
 Notation "'★' e" := (Load e) (at level 30) : lang_scope.
 Notation "e1 '<-' e2" := (Store e1 e2) (at level 60) : lang_scope.
@@ -49,8 +47,12 @@ Notation "'new' e" := (Alloc e) (at level 60) : lang_scope.
 Notation "e1 '+' e2" := (Plus e1 e2) : lang_scope.
 Notation "e1 '≤' e2" := (Le e1 e2) : lang_scope.
 Notation "e1 '<' e2" := (Lt e1 e2) : lang_scope.
+
 Coercion LitNat : nat >-> expr.
+Coercion LitNatV : nat >-> val.
 Coercion Loc : loc >-> expr.
+Coercion LocV : loc >-> val.
+Coercion App : expr >-> Funclass.
 
 Section suger.
 Context {Σ : iFunctor}.
